Simplify sinv library

nola/iris/sinv.v
@@ -28,146 +28,120 @@ Section sinv.
   Implicit Type Px : FML $oi Σ.
 
   (** Simple invariant token *)
-  Local Definition sinv_itok_def i Px : iProp Σ :=
+  Local Definition sinv_tok_def i Px : iProp Σ :=
     own sinv_name (gmap_view_frag i DfracDiscarded (to_agree Px)).
-  Local Lemma sinv_itok_aux : seal sinv_itok_def. Proof. by eexists. Qed.
-  Definition sinv_itok := sinv_itok_aux.(unseal).
-  Local Lemma sinv_itok_unseal : sinv_itok = sinv_itok_def.
+  Local Lemma sinv_tok_aux : seal sinv_tok_def. Proof. by eexists. Qed.
+  Definition sinv_tok := sinv_tok_aux.(unseal).
+  Local Lemma sinv_tok_unseal : sinv_tok = sinv_tok_def.
   Proof. exact: seal_eq. Qed.
-
-  (** Simple invariant token with the index hidden *)
-  Definition sinv_tok Px : iProp Σ := ∃ i, sinv_itok i Px.
 
   (** Authoritative token *)
   Local Definition sinv_auth_tok M :=
     own sinv_name (gmap_view_auth (DfracOwn 1) (to_agree <$> M)).
   (** World satisfaction *)
-  Definition sinv_iwsat_def sm : iProp Σ :=
+  Definition sinv_wsat_def sm : iProp Σ :=
     □ (∀ i Px Qx, Px ≡ Qx -∗ sm i Px -∗ sm i Qx) ∗
     ∃ M, sinv_auth_tok M ∗ [∗ map] i ↦ Px ∈ M, sm i Px.
-  Local Lemma sinv_iwsat_aux : seal sinv_iwsat_def. Proof. by eexists. Qed.
-  Definition sinv_iwsat := sinv_iwsat_aux.(unseal).
-  Local Lemma sinv_iwsat_unseal : sinv_iwsat = sinv_iwsat_def.
+  Local Lemma sinv_wsat_aux : seal sinv_wsat_def. Proof. by eexists. Qed.
+  Definition sinv_wsat := sinv_wsat_aux.(unseal).
+  Local Lemma sinv_wsat_unseal : sinv_wsat = sinv_wsat_def.
   Proof. exact: seal_eq. Qed.
 End sinv.
-(** World satisfaction whose semantics ignores the index *)
-Notation sinv_wsat' FML sm := (sinv_iwsat (FML:=FML) (λ _, sm)).
-Notation sinv_wsat sm := (sinv_wsat' _ sm).
 
 Section sinv.
   Context `{!sinvGS FML Σ}.
   Implicit Type Px : FML $oi Σ.
   Implicit Type (i : positive) (I : gset positive).
 
-  (** [sinv_itok] and [sinv_tok] are non-expansive *)
-  #[export] Instance sinv_itok_ne {i} : NonExpansive (sinv_itok i).
-  Proof. rewrite sinv_itok_unseal. solve_proper. Qed.
-  #[export] Instance sinv_itok_proper {i} : Proper ((≡) ==> (⊣⊢)) (sinv_itok i).
+  (** [sinv_tok] is non-expansive *)
+  #[export] Instance sinv_tok_ne {i} : NonExpansive (sinv_tok i).
+  Proof. rewrite sinv_tok_unseal. solve_proper. Qed.
+  #[export] Instance sinv_tok_proper {i} : Proper ((≡) ==> (⊣⊢)) (sinv_tok i).
   Proof. apply ne_proper, _. Qed.
-  #[export] Instance sinv_tok_ne : NonExpansive sinv_tok.
-  Proof. solve_proper. Qed.
-  #[export] Instance sinv_tok_proper: Proper ((≡) ==> (⊣⊢)) sinv_tok.
-  Proof. solve_proper. Qed.
-  (** [sinv_itok] and [sinv_tok] are persistent *)
-  #[export] Instance sinv_itok_persistent {i Px} : Persistent (sinv_itok i Px).
-  Proof. rewrite sinv_itok_unseal. exact _. Qed.
-  #[export] Instance sinv_tok_persistent {Px} : Persistent (sinv_tok Px).
-  Proof. exact _. Qed.
-  (** [sinv_itok] and [sinv_tok] are timeless for discrete formulas *)
-  #[export] Instance sinv_itok_timeless `{!Discrete Px} {i} :
-    Timeless (sinv_itok i Px).
-  Proof. rewrite sinv_itok_unseal /sinv_itok_def /gmap_view_frag. exact _. Qed.
-  #[export] Instance sinv_tok_timeless `{!Discrete Px} : Timeless (sinv_tok Px).
-  Proof. exact _. Qed.
+  (** [sinv_tok] is persistent *)
+  #[export] Instance sinv_tok_persistent {i Px} : Persistent (sinv_tok i Px).
+  Proof. rewrite sinv_tok_unseal. exact _. Qed.
+  (** [sinv_tok] is timeless for discrete formulas *)
+  #[export] Instance sinv_tok_timeless `{!Discrete Px} {i} :
+    Timeless (sinv_tok i Px).
+  Proof. rewrite sinv_tok_unseal /sinv_tok_def /gmap_view_frag. exact _. Qed.
 
-  (** [sinv_iwsat] is non-expansive *)
-  #[export] Instance sinv_iwsat_ne {n} :
+  (** [sinv_wsat] is non-expansive *)
+  #[export] Instance sinv_wsat_ne {n} :
     Proper (pointwise_relation _ (pointwise_relation _ (≡{n}≡)) ==> (≡{n}≡))
-      sinv_iwsat.
-  Proof. rewrite sinv_iwsat_unseal. solve_proper. Qed.
-  #[export] Instance sinv_iwsat_proper :
-    Proper (pointwise_relation _ (pointwise_relation _ (≡)) ==> (≡)) sinv_iwsat.
-  Proof. rewrite sinv_iwsat_unseal. solve_proper. Qed.
+      sinv_wsat.
+  Proof. rewrite sinv_wsat_unseal. solve_proper. Qed.
+  #[export] Instance sinv_wsat_proper :
+    Proper (pointwise_relation _ (pointwise_relation _ (≡)) ==> (≡)) sinv_wsat.
+  Proof. rewrite sinv_wsat_unseal. solve_proper. Qed.
 
-  (** [sinv_iwsat] is timeless if [sm] is always timeless
+  (** [sinv_wsat] is timeless if [sm] is always timeless
     and the underlying ofe is discrete *)
-  #[export] Instance sinv_iwsat_timeless
+  #[export] Instance sinv_wsat_timeless
     `{!OfeDiscrete (FML $oi Σ), !∀ i Px, Timeless (sm i Px)} :
-    Timeless (sinv_iwsat sm).
-  Proof. rewrite sinv_iwsat_unseal. exact _. Qed.
+    Timeless (sinv_wsat sm).
+  Proof. rewrite sinv_wsat_unseal. exact _. Qed.
 
-  (** Lemma for [sinv_itok_alloc] *)
+  (** Lemma for [sinv_tok_alloc] *)
   Local Lemma sinv_auth_tok_alloc {M i Px} : i ∉ dom M →
-    sinv_auth_tok M ==∗ sinv_auth_tok (<[i:=Px]> M) ∗ sinv_itok i Px.
+    sinv_auth_tok M ==∗ sinv_auth_tok (<[i:=Px]> M) ∗ sinv_tok i Px.
   Proof.
-    move=> /not_elem_of_dom eq. iIntros "●". rewrite sinv_itok_unseal -own_op.
+    move=> /not_elem_of_dom eq. iIntros "●". rewrite sinv_tok_unseal -own_op.
     iApply own_update; [|done]. rewrite fmap_insert.
     apply gmap_view_alloc; [|done..]. by rewrite lookup_fmap eq.
   Qed.
-  (** Allocate [sinv_itok] *)
-  Lemma sinv_itok_alloc {sm} Px :
-    sinv_iwsat sm -∗ ∃ I, ∀ i, ⌜i ∉ I⌝ ==∗
-      sinv_itok i Px ∗ (sm i Px -∗ sinv_iwsat sm).
-  Proof.
-    rewrite sinv_iwsat_unseal. iIntros "[Ne[%M[● M]]]". iExists (dom M).
-    iIntros (i ?). iMod (sinv_auth_tok_alloc with "●") as "[● #i]"; [done|].
-    iModIntro. iSplitR; [by rewrite sinv_itok_unseal|]. iIntros "Px".
-    iFrame "Ne ●". iApply (big_sepM_insert_2 with "Px M").
-  Qed.
   (** Allocate [sinv_tok] *)
   Lemma sinv_tok_alloc {sm} Px :
-    sinv_wsat sm ==∗ sinv_tok Px ∗ (sm Px -∗ sinv_wsat sm).
+    sinv_wsat sm -∗ ∃ I, ∀ i, ⌜i ∉ I⌝ ==∗
+      sinv_tok i Px ∗ (sm i Px -∗ sinv_wsat sm).
   Proof.
-    iIntros "W". iDestruct (sinv_itok_alloc with "W") as (?) "big".
-    iMod ("big" with "[]") as "[? $]". { iPureIntro. apply is_fresh. }
-    iModIntro. by iExists _.
+    rewrite sinv_wsat_unseal. iIntros "[Ne[%M[● M]]]". iExists (dom M).
+    iIntros (i ?). iMod (sinv_auth_tok_alloc with "●") as "[● #i]"; [done|].
+    iModIntro. iSplitR; [by rewrite sinv_tok_unseal|]. iIntros "Px".
+    iFrame "Ne ●". iApply (big_sepM_insert_2 with "Px M").
   Qed.
 
-  (** Lemma for [sinv_itok_acc] *)
+  (** Lemma for [sinv_tok_acc] *)
   Local Lemma sinv_auth_tok_lookup {M i Px} :
-    sinv_auth_tok M -∗ sinv_itok i Px -∗ ∃ Px', ⌜M !! i = Some Px'⌝ ∗ Px ≡ Px'.
+    sinv_auth_tok M -∗ sinv_tok i Px -∗ ∃ Px', ⌜M !! i = Some Px'⌝ ∗ Px ≡ Px'.
   Proof.
-    rewrite sinv_itok_unseal. iIntros "● i".
+    rewrite sinv_tok_unseal. iIntros "● i".
     iDestruct (own_valid_2 with "● i") as "✓".
     rewrite gmap_view_both_validI_total. iDestruct "✓" as (? _ _ eq) "[_ in]".
     move: eq. rewrite lookup_fmap. case: (M !! i); [|done]=> Px' [<-].
     iExists Px'. iSplit; [done|]. by rewrite to_agree_includedI.
   Qed.
-  (** Access via [sinv_itok] *)
-  Lemma sinv_itok_acc {i sm Px} :
-    sinv_itok i Px -∗ sinv_iwsat sm -∗ sm i Px ∗ (sm i Px -∗ sinv_iwsat sm).
+  (** Access via [sinv_tok] *)
+  Lemma sinv_tok_acc {i sm Px} :
+    sinv_tok i Px -∗ sinv_wsat sm -∗ sm i Px ∗ (sm i Px -∗ sinv_wsat sm).
   Proof.
-    rewrite sinv_iwsat_unseal. iIntros "i [#Ne[%M[● M]]]".
+    rewrite sinv_wsat_unseal. iIntros "i [#Ne[%M[● M]]]".
     iDestruct (sinv_auth_tok_lookup with "● i") as (Px' eq) "#≡".
     iDestruct (big_sepM_lookup_acc with "M") as "[Px' →M]"; [done|].
     iDestruct ("Ne" with "[] Px'") as "$"; [by iApply internal_eq_sym|].
     iIntros "Px". iDestruct ("Ne" with "≡ Px") as "Px'". iFrame "Ne ●".
     by iApply "→M".
   Qed.
-  (** Access via [sinv_tok] *)
-  Lemma sinv_tok_acc {sm Px} :
-    sinv_tok Px -∗ sinv_wsat sm -∗ sm Px ∗ (sm Px -∗ sinv_wsat sm).
-  Proof. iIntros "[%i i]". iApply (sinv_itok_acc with "i"). Qed.
 End sinv.
 
-(** Lemma for [sinv_iwsat_alloc] *)
+(** Lemma for [sinv_wsat_alloc] *)
 Local Lemma sinv_auth_tok_alloc_empty `{!sinvGpreS FML Σ} :
   ⊢ |==> ∃ _ : sinvGS FML Σ, sinv_auth_tok ∅.
 Proof.
   iMod (own_alloc (gmap_view_auth (DfracOwn 1) ∅)) as (γ) "●".
   { apply gmap_view_auth_valid. } { iModIntro. by iExists (SinvGS _ _ _ γ). }
 Qed.
-(** Allocate [sinv_iwsat] *)
-Lemma sinv_iwsat_alloc' `{!sinvGpreS FML Σ} :
+(** Allocate [sinv_wsat] *)
+Lemma sinv_wsat_alloc' `{!sinvGpreS FML Σ} :
   ⊢ |==> ∃ _ : sinvGS FML Σ,
-    ∀ sm, □ (∀ i Px Qx, Px ≡ Qx -∗ sm i Px -∗ sm i Qx) -∗ sinv_iwsat sm.
+    ∀ sm, □ (∀ i Px Qx, Px ≡ Qx -∗ sm i Px -∗ sm i Qx) -∗ sinv_wsat sm.
 Proof.
   iMod sinv_auth_tok_alloc_empty as (?) "●". iModIntro. iExists _.
-  iIntros (?) "Ne". rewrite sinv_iwsat_unseal. by iFrame.
+  iIntros (?) "Ne". rewrite sinv_wsat_unseal. by iFrame.
 Qed.
-Lemma sinv_iwsat_alloc `{!sinvGpreS FML Σ} :
-  ⊢ |==> ∃ _ : sinvGS FML Σ, ∀ sm, ⌜∀ i, NonExpansive (sm i)⌝ -∗ sinv_iwsat sm.
+Lemma sinv_wsat_alloc `{!sinvGpreS FML Σ} :
+  ⊢ |==> ∃ _ : sinvGS FML Σ, ∀ sm, ⌜∀ i, NonExpansive (sm i)⌝ -∗ sinv_wsat sm.
 Proof.
-  iMod sinv_iwsat_alloc' as (?) "W". iModIntro. iExists _. iIntros (??).
+  iMod sinv_wsat_alloc' as (?) "W". iModIntro. iExists _. iIntros (??).
   iApply "W". iIntros "!> %%% eqv ?". by iRewrite -"eqv".
 Qed.
